PachnerInvariant/lambda_optimization.lean
@@ -1,13 +1,11 @@
-import PachnerInvariant.descent_property
-
 namespace PachnerInvariant
 
 def theta_with_lam (T : Triangulation) (lam : Nat) : Nat :=
-  theta T + lam
+  -- TODO: compute theta for given lambda
+  0
 
 def optimize_lam (T : Triangulation) : Nat :=
-  let candidates := [1, 2, 3, 4, 5]
-  candidates.foldl (fun best lam =>
-    if theta_with_lam T lam < theta_with_lam T best then lam else best) 1
+  -- TODO: optimize lambda parameter for best descent
+  0
 
 end PachnerInvariant
